Finish encode bot as bot

Lib/Encode_Nat/Encode_Nat.thy
@@ -12,6 +12,7 @@ theory Encode_Nat
     "HOL-Library.List_Lexorder"
     "HOL-Library.Product_Lexorder"
     "HOL-Library.Multiset"
+    "HOL-Library.Option_ord"
     "HOL-Eisbach.Eisbach"
     "HOL-Eisbach.Eisbach_Tools"
     Test
@@ -25,6 +26,13 @@ theory Encode_Nat
     "function_nat_rewrite_correctness" :: thy_goal
 begin
 
+declare [[ML_print_depth = 50]]
+
+datatype ('a, 'b) keyed_list_tree =
+  KLeaf |
+  KNode "(('a, 'b) keyed_list_tree)" 'a "('b list)" "(('a, 'b) keyed_list_tree)"
+
+type_synonym pair_repr = nat
 
 instantiation char :: order_bot
 begin
@@ -52,11 +60,77 @@ next
   then show ?case
     unfolding bot_char_def less_eq_char_def by (cases a, fastforce)
 qed
-
 end
 
+instantiation tree :: (order) order_bot
+begin
 
-type_synonym pair_repr = nat
+fun less_eq_tree :: "'a tree \<Rightarrow> 'a tree \<Rightarrow> bool" where
+  "less_eq_tree \<langle>\<rangle> _ \<longleftrightarrow> True"
+| "less_eq_tree _ \<langle>\<rangle> \<longleftrightarrow> False"
+| "less_eq_tree \<langle>l1, a1, r1\<rangle> \<langle>l2, a2, r2\<rangle> \<longleftrightarrow>
+    (l1 \<le> l2 \<and> r1 \<le> r2 \<and> a1 \<le> a2)"
+
+definition less_tree :: "'a tree \<Rightarrow> 'a tree \<Rightarrow> bool" where
+  "less_tree t1 t2 = (t1 \<le> t2 \<and> \<not> t2 \<le> t1)"
+
+definition bot_tree :: "'a tree" where
+  "bot_tree = \<langle>\<rangle>"
+
+instance
+proof(standard, goal_cases)
+  case 1 show ?case using less_tree_def by simp
+next
+  case (2 t) show ?case by(induction t; simp)
+next
+  case (3 t1 t2 t3) thus ?case
+    by(induction t1 t3 arbitrary: t2 rule: less_eq_tree.induct; force elim: less_eq_tree.elims)
+next
+  case (4 t1 t2) thus ?case
+    by(induction t1 t2 rule: less_eq_tree.induct; force elim: less_eq_tree.elims)
+next
+  case (5 a)
+  then show ?case
+    unfolding bot_tree_def less_eq_tree.simps by simp
+qed
+end
+
+instantiation keyed_list_tree :: (order, order) order_bot
+begin
+
+fun less_eq_keyed_list_tree :: "('a, 'b) keyed_list_tree \<Rightarrow> ('a, 'b) keyed_list_tree \<Rightarrow> bool" where
+  "less_eq_keyed_list_tree KLeaf _ \<longleftrightarrow> True"
+| "less_eq_keyed_list_tree _ KLeaf \<longleftrightarrow> False"
+| "less_eq_keyed_list_tree (KNode l1 a1 bs1 r1) (KNode l2 a2 bs2 r2) \<longleftrightarrow>
+    (l1 \<le> l2 \<and> r1 \<le> r2 \<and> a1 \<le> a2 \<and> bs1 \<le> bs2)"
+
+definition less_keyed_list_tree :: "('a, 'b) keyed_list_tree \<Rightarrow> ('a, 'b) keyed_list_tree \<Rightarrow> bool"
+  where
+    "less_keyed_list_tree t1 t2 = (t1 \<le> t2 \<and> \<not> t2 \<le> t1)"
+
+definition bot_keyed_list_tree :: "('a, 'b) keyed_list_tree" where
+  "bot_keyed_list_tree = KLeaf"
+
+instance
+proof(standard, goal_cases)
+  case 1 show ?case using less_keyed_list_tree_def by simp
+next
+  case (2 t) show ?case by(induction t; simp)
+next
+  case (3 t1 t2 t3) thus ?case
+    by(induction t1 t3 arbitrary: t2 rule: less_eq_keyed_list_tree.induct;
+        force elim: less_eq_keyed_list_tree.elims)
+next
+  case (4 t1 t2) thus ?case
+    by(induction t1 t2 rule: less_eq_keyed_list_tree.induct;
+        force elim: less_eq_keyed_list_tree.elims)
+next
+  case (5 a)
+  then show ?case
+    unfolding bot_keyed_list_tree_def less_eq_keyed_list_tree.simps by simp
+qed
+end
+
 
 fun atomic :: "nat \<Rightarrow> pair_repr" where
   "atomic a = a"
@@ -73,9 +147,6 @@ fun sndP :: "pair_repr \<Rightarrow> pair_repr" where
 
 ML_file \<open>./Encode_Nat.ML\<close>
 
-
-fun size_pair_repr :: "pair_repr \<Rightarrow> nat" where
-  "size_pair_repr v = v"
 
 lemma prod_decode_less:
   assumes "v < v'"
@@ -98,208 +169,151 @@ lemma snd_prod_encode_lt: "a > 0 \<Longrightarrow> b < prod_encode (a, b)"
 corollary snd_prod_decode_lt_intro:
   assumes "fstP v \<noteq> 0"
   shows "snd (prod_decode v) < v"
-proof -
-  obtain x y where xyv: "prod_decode v = (x, y)" by fastforce
-  with assms have "y < prod_encode (x, y)" using snd_prod_encode_lt by simp
-  then show ?thesis using prod_decode_inverse[of v] unfolding xyv by simp
-qed
-
-declare [[ML_print_depth = 50]]
+  by (metis assms fstP.simps gr0I prod.collapse snd_prod_encode_lt prod_decode_inverse)
 
 
 datatype_nat_encode nat
-declare enc_nat.simps [simp del]
+
+lemma enc_nat_bot: "enc_nat bot = bot"
+  by simp
 
 datatype_nat_encode list
 declare enc_list.simps [simp del]
 
-value "bot::bool"
-value "0 = (bot::nat)"
-thm bot_nat_def
-lemma "(0::nat) = (bot::nat)"
-  by (simp add: bot_nat_def)
-
-
-ML \<open>
-val a = @{term "0::nat"};
-val b = @{term "bot::nat"};
-
-val goal = Logic.mk_equals (a, b);
-val ctxt = @{context};
-
-\<close>
+lemma enc_list_bot: "enc_list enc_'a bot = bot"
+  by(simp add: enc_list.simps prod_encode_def bot_list_def bot_nat_def)
 
 datatype_nat_encode bool
 declare enc_bool.simps [simp del]
 
-term "Product_Type.bool.case_bool a b c"
-term "case_list a b c"
-term "case_bool "
-
-value "enc_bool bot = bot"
+lemma enc_bool_bot: "enc_bool bot = bot"
+  by(simp add: enc_bool.simps prod_encode_def bot_nat_def)
 
 datatype_nat_encode char
 declare enc_char.simps [simp del]
 
+lemma enc_char_bot: "enc_char bot = bot"
+  by(simp add: enc_char.simps enc_bool.simps prod_encode_def bot_nat_def bot_char_def)
+
 datatype_nat_encode prod
-declare enc_prod.simps [simp del] thm enc_prod.simps
+declare enc_prod.simps [simp del]
+
+lemma enc_prod_bot:
+  assumes "enc_'a bot = bot"
+    and "enc_'b bot = bot"
+  shows "enc_prod enc_'a enc_'b bot = bot"
+  by (simp add: enc_prod.simps prod_encode_def bot_nat_def bot_prod_def assms)
 
 datatype_nat_encode tree
 declare enc_tree.simps [simp del]
 
-
-datatype ('a, 'b) keyed_list_tree =
-  KLeaf |
-  KNode "(('a, 'b) keyed_list_tree)" 'a "('b list)" "(('a, 'b) keyed_list_tree)"
-
+lemma enc_tree_bot: "enc_tree enc_'a bot = bot"
+  by (simp add: enc_tree.simps prod_encode_def bot_nat_def bot_tree_def)
 
 datatype_nat_encode keyed_list_tree
 declare enc_keyed_list_tree.simps [simp del]
-thm enc_keyed_list_tree.simps
 
-datatype 'a forest =
-  FLeaf |
-  FNode "(('a forest) list)"
+lemma enc_keyed_list_tree_bot: "enc_keyed_list_tree enc_'a enc_'b bot = bot"
+  by (simp add: enc_keyed_list_tree.simps prod_encode_def bot_nat_def bot_keyed_list_tree_def)
 
+
+(* TODO: Do we need similar lemmas for other data types? *)
 lemma enc_List_list_cong[fundef_cong]:
   assumes "xs = ys"
     and "\<And>x. x \<in> set ys \<Longrightarrow> enc\<^sub>a x = enc\<^sub>b x"
   shows "enc_list enc\<^sub>a xs = enc_list enc\<^sub>b ys"
   using assms by (induction xs arbitrary: ys; auto simp add: enc_list.simps)
 
-datatype_nat_encode forest
-declare enc_forest.simps [simp del]
-thm enc_forest.simps
 
 method decode_termination for t =
   relation t, auto;
   (auto intro!: prod_decode_less snd_prod_decode_lt_intro)?
 
 
-
-
 datatype_nat_decode nat
 termination by (decode_termination "measure id")
-thm dec_nat.simps
 
 datatype_nat_decode list
 termination by (decode_termination "measure snd")
 declare dec_list.simps[simp del]
-lemmas [simp] = dec_list.simps[of _ "prod_encode _"]
+  (* Why? *)
+lemmas dec_list_prod_encode_simp[simp] = dec_list.simps[of _ "prod_encode _"]
+
 thm dec_list.simps
-
-datatype_nat_decode prod
-termination by (decode_termination "measure (snd o snd)")
-declare dec_prod.simps[simp del]
-lemmas [simp] = dec_prod.simps[of _ _ "prod_encode _"]
-thm dec_prod.simps
-
-datatype_nat_decode tree
-termination by (decode_termination "measure snd")
-declare dec_tree.simps[simp del]
-lemmas [simp] = dec_tree.simps[of _ "prod_encode _"]
-thm dec_tree.simps
-
-datatype_nat_decode keyed_list_tree
-termination by (decode_termination "measure (snd o snd)")
-declare dec_keyed_list_tree.simps[simp del]
-lemmas [simp] = dec_keyed_list_tree.simps[of _ _ "prod_encode _"]
-thm dec_keyed_list_tree.simps
-
-
-inductive_set
-  subpairings :: "pair_repr \<Rightarrow> pair_repr set"
-  for x
-  where
-    "x \<in> subpairings x"
-  | "t \<in> subpairings x \<Longrightarrow> fstP t \<in> subpairings x"
-  | "t \<in> subpairings x \<Longrightarrow> sndP t \<in> subpairings x"
-
-lemma
-  shows subpairings_fstP_imp: "a \<in> subpairings (fstP x) \<Longrightarrow> a \<in> subpairings x"
-    and subpairings_sndP_imp: "a \<in> subpairings (sndP x) \<Longrightarrow> a \<in> subpairings x"
-  apply(simp, all \<open>induction rule: subpairings.induct\<close>)
-  using subpairings.intros by simp+
-
-lemma subpairings_le: "a \<in> subpairings x \<Longrightarrow> a \<le> x"
-  apply(induction rule: subpairings.induct)
-  using prod_decode_lte[of _ x] by simp+
-
-lemma dec_List_list_cong[fundef_cong]:
-  assumes "x = y"
-    and "\<And>t. t \<in> subpairings y \<Longrightarrow> dec\<^sub>a t = dec\<^sub>b t"
-  shows "dec_list dec\<^sub>a x = dec_list dec\<^sub>b y"
-  unfolding assms(1)
-  using assms(2)
-  apply (induction dec\<^sub>a y rule: dec_list.induct)
-  subgoal for _ v
-    apply (unfold dec_list.simps[of _ v])
-    using subpairings.intros
-      \<comment> \<open>specialized for the recursive constructor field:\<close>
-      subpairings_sndP_imp[OF subpairings_sndP_imp[of _ "sndP v"]]
-    by presburger
-  done
-
-datatype_nat_decode forest
-termination
-  using subpairings_le snd_prod_decode_lt_intro
-  by (decode_termination "measure snd", fastforce)
-
-
-declare dec_forest.simps[simp del]
-lemmas [simp] = dec_forest.simps[of _ "prod_encode _"]
-thm dec_forest.simps
-
-
-method wellbehavedness_case
-  uses assms enc_simps uses_wellbehaved =
-  \<comment> \<open>Unfold the encoder applied to the universally argument once.\<close>
-  subst enc_simps,
-  \<comment> \<open>Type variables are assumed to be well-behaved.\<close>
-  insert assms,
-  \<comment> \<open>Wellbehavedness of other data types used by constructors must be provided.\<close>
-  insert uses_wellbehaved,
-  auto
-
-method wellbehavedness
-  uses induct_rule assms enc_simps uses_wellbehaved =
-  (intro ext,
-    \<comment> \<open>\<open>\<dots>\<close>but \<open>induction\<close> still refuses to run structural induction correctly when\<close>
-    \<comment> \<open>the goal is universally quantified and there are no assumptions.\<close>
-    \<comment> \<open>Outside of Eisbach, \<^bold>\<open>subgoal apply\<close> \<open>(induction rule: induct_rule)\<close>\<close>
-    \<comment> \<open>does the trick. This is the shortest replacement I found.\<close>
-    insert TrueI, match premises in True \<Rightarrow> \<open>induction rule: induct_rule\<close>);
-  (solves \<open>wellbehavedness_case
-           assms: assms enc_simps: enc_simps uses_wellbehaved: uses_wellbehaved\<close>
-    \<comment> \<open>If that approach didn't work, return the original induction case\<close>
-    )?
-
-ML \<open>
-val T = @{typ "'a list"};
-is_Type T;
-is_TFree T;
-is_TVar T;
-val [T'] = dest_Type T |> snd;
-is_Type T;
-is_TFree T;
-is_TVar T;
-
-\<close>
-
 
 datatype_nat_decode bool
 termination by (decode_termination "measure id")
 declare dec_bool.simps[simp del]
+  (* Why? *)
+lemmas dec_bool_prod_encode_simp[simp] = dec_bool.simps[of "prod_encode _"]
 
-thm dec_bool.simps
+datatype_nat_decode char
+termination by (decode_termination "measure id")
+declare dec_char.simps[simp del]
+  (* Why? *)
+lemmas dec_char_prod_encode_simp[simp] = dec_char.simps[of "prod_encode _"]
 
-datatype_nat_wellbehaved bool
-  by(intro ext, simp add: dec_bool.simps enc_bool.simps split:bool.split)
-thm encoding_bool_wellbehaved
+datatype_nat_decode prod
+termination by (decode_termination "measure (snd o snd)")
+declare dec_prod.simps[simp del]
+  (* Why? *)
+lemmas dec_prod_prod_encode_simp[simp] = dec_prod.simps[of _ _ "prod_encode _"]
+
+datatype_nat_decode tree
+termination by (decode_termination "measure snd")
+declare dec_tree.simps[simp del]
+  (* Why? *)
+lemmas dec_tree_prod_encode_simp[simp] = dec_tree.simps[of _ "prod_encode _"]
+
+datatype_nat_decode keyed_list_tree
+termination by (decode_termination "measure (snd o snd)")
+declare dec_keyed_list_tree.simps[simp del]
+  (* Why? *)
+lemmas dec_keyed_list_tree_prod_encode_simp[simp]
+  = dec_keyed_list_tree.simps[of _ _ "prod_encode _"]
+
+
+inductive_set subpairings :: "pair_repr \<Rightarrow> pair_repr set" for x where
+  "x \<in> subpairings x"
+| "t \<in> subpairings x \<Longrightarrow> fstP t \<in> subpairings x"
+| "t \<in> subpairings x \<Longrightarrow> sndP t \<in> subpairings x"
+
+lemma
+  shows subpairings_fstP_imp: "a \<in> subpairings (fstP x) \<Longrightarrow> a \<in> subpairings x"
+    and subpairings_sndP_imp: "a \<in> subpairings (sndP x) \<Longrightarrow> a \<in> subpairings x"
+   apply(simp, all \<open>induction rule: subpairings.induct\<close>)
+  using subpairings.intros by simp+
+
+(* TODO: Do we need similar lemmas for other data types? *)
+lemma dec_List_list_cong[fundef_cong]:
+  assumes "x = y"
+    and "\<And>t. t \<in> subpairings y \<Longrightarrow> dec\<^sub>a t = dec\<^sub>b t"
+  shows "dec_list dec\<^sub>a x = dec_list dec\<^sub>b y"
+  unfolding assms(1) using assms(2)
+  by (induction dec\<^sub>a y rule: dec_list.induct;
+      metis subpairings_sndP_imp dec_list.simps subpairings.intros(1) subpairings.intros(2))
+
+(* No longer working. TODO? *)
+method wellbehavedness_case
+  uses assms enc_simps uses_wellbehaved =
+  subst enc_simps,
+  insert assms,
+  insert uses_wellbehaved,
+  auto
+
+(* No longer working. TODO? *)
+method wellbehavedness
+  uses induct_rule assms enc_simps uses_wellbehaved =
+  (intro ext, insert TrueI, match premises in True \<Rightarrow> \<open>induction rule: induct_rule\<close>);
+  (solves \<open>wellbehavedness_case
+            assms: assms enc_simps: enc_simps uses_wellbehaved: uses_wellbehaved\<close>)?
+
 
 datatype_nat_wellbehaved nat
   using dec_nat.simps enc_nat.simps by fastforce
-thm encoding_nat_wellbehaved
+
+datatype_nat_wellbehaved bool
+  by(intro ext, simp add: dec_bool.simps enc_bool.simps split:bool.split)
 
 datatype_nat_wellbehaved list
   apply(intro ext)
@@ -308,14 +322,16 @@ datatype_nat_wellbehaved list
     by(induction x rule: list.induct; simp add: enc_list.simps)
   done
 
+datatype_nat_wellbehaved char
+  using encoding_bool_wellbehaved[THEN pointfree_idE]
+  by(intro ext, simp add: dec_char.simps enc_char.simps split:char.split)
+
 datatype_nat_wellbehaved prod
   apply(intro ext)
   subgoal for x
     using assms[THEN pointfree_idE]
     by(induction x rule: prod.induct; simp add: enc_prod.simps)
   done
-
-thm encoding_prod_wellbehaved
 
 datatype_nat_wellbehaved tree
   apply(intro ext)
@@ -324,8 +340,6 @@ datatype_nat_wellbehaved tree
     by(induction x rule: tree.induct; simp add: enc_tree.simps)
   done
 
-thm encoding_tree_wellbehaved
-
 datatype_nat_wellbehaved keyed_list_tree
   apply(intro ext)
   subgoal for x
@@ -333,22 +347,6 @@ datatype_nat_wellbehaved keyed_list_tree
     using encoding_list_wellbehaved[OF assms(2)] assms(1)
     by (simp add: enc_keyed_list_tree.simps pointfree_idE)+
   done
-
-thm encoding_keyed_list_tree_wellbehaved
-
-datatype_nat_wellbehaved forest
-  apply(intro ext)
-  subgoal for x
-    apply(induction x rule: forest.induct)
-    using encoding_list_wellbehaved[OF assms(1)]
-    apply (simp add: enc_forest.simps pointfree_idE)
-    subgoal for x
-      apply (induction x rule: list.induct)
-      by(simp add: enc_list.simps enc_forest.simps)+
-    done
-  done
-
-thm encoding_forest_wellbehaved
 
 method natfn_correctness
   methods induct_rule
@@ -372,19 +370,13 @@ lemma reverset_correct: "reverset l [] = rev l"
   by (simp add: reverset_rev)
 
 function_nat_rewrite reverset
-thm reverset_nat.simps
-
 
 function_nat_rewrite_correctness reverset
-  apply(induction arg\<^sub>1 arg\<^sub>2 rule: reverset.induct)
-  apply(all \<open>subst reverset_nat.simps\<close>)
-  subgoal
-    apply(subst enc_list.simps)
-    using encoding_list_wellbehaved[OF assms(1)]
-    by(simp add: assms pointfree_idE )
-  subgoal
-    by(simp add: enc_list.simps)
-  done
+  by (natfn_correctness \<open>induct arg\<^sub>1 arg\<^sub>2 rule: reverset.induct\<close>
+      assms: assms
+      simps_nat: reverset_nat.simps
+      enc_simps: enc_list.simps
+      args_wellbehaved: encoding_list_wellbehaved[OF assms(1), THEN pointfree_idE])
 
 thm reverset_nat_equiv
 
@@ -403,66 +395,39 @@ corollary prefixest_correct: "prefixest a [] = rev (prefixes a)"
   by (simp add: prefixest_prefixes)
 
 function_nat_rewrite prefixest
-thm prefixest_nat.simps
-thm prefixest.induct
 
 function_nat_rewrite_correctness prefixest
-  using assms
-  apply(induction arg\<^sub>1 arg\<^sub>2 rule: prefixest.induct; subst prefixest_nat.simps)
-  using encoding_list_wellbehaved[OF encoding_list_wellbehaved, OF assms(1), THEN pointfree_idE]
-  by(simp add: enc_list.simps Let_def)+
-
-(* or
   by (natfn_correctness \<open>induct arg\<^sub>1 arg\<^sub>2 rule: prefixest.induct\<close>
       assms: assms
       simps_nat: prefixest_nat.simps
-      enc_simps: enc_List_list.simps
+      enc_simps: enc_list.simps
       args_wellbehaved:
-      List_list_wellbehaved[OF List_list_wellbehaved, OF assms(1), THEN pointfree_idE])
-*)
-
-thm prefixest_nat_equiv
-
+      encoding_list_wellbehaved[OF encoding_list_wellbehaved, OF assms(1), THEN pointfree_idE])
 
 fun prefixes2 where
   "prefixes2 [] ps = reverset ([] # ps) []"
 | "prefixes2 (a # b) ps = prefixes2 b ((a # b) # ps)"
 
 function_nat_rewrite prefixes2
-thm prefixes2_nat.simps back_subst[of _ "x # xs"]
 
+lemma dec_list_bot: "dec_list dec_'a bot = bot"
+  by(simp add: dec_list.simps prod_decode_def prod_decode_aux.simps bot_list_def)
 
 function_nat_rewrite_correctness prefixes2
   using assms
   apply(induction arg\<^sub>1 arg\<^sub>2 rule: prefixes2.induct; subst prefixes2_nat.simps)
   subgoal for ps
-    using
-      reverset_nat_equiv[OF encoding_list_wellbehaved, OF assms, of "[] # ps" "[]"]
+    using reverset_nat_equiv[
+        OF encoding_list_wellbehaved,
+        OF assms(1),
+        OF dec_list_bot,
+        of "[] # ps" "[]"]
     by(simp add: enc_list.simps)
   by(simp add: enc_list.simps Let_def)
-    (*
-  apply (natfn_correctness \<open>induct arg\<^sub>1 arg\<^sub>2 rule: prefixes2.induct\<close>
-      assms: assms
-      simps_nat: prefixes2_nat.simps
-      enc_simps: enc_List_list.simps
-      dels: reverset.simps
-      args_wellbehaved: List_list_wellbehaved[OF List_list_wellbehaved, OF assms(1), THEN pointfree_idE]
-      List_list_wellbehaved[OF assms(1), THEN pointfree_idE])
-  subgoal for ps
-    \<comment> \<open>We need to explicitly instantiate the equivalence rule for the called function.\<close>
-    \<comment> \<open>Figuring out exactly what fact to supply is very mechanic:\<close>
-    \<comment> \<open>The \<open>wellbehaved\<close> fact(s) can be fetched from the function, while the arguments\<close>
-    \<comment> \<open>appear in the same order they do in the simp rule that generates the subgoal.\<close>
-    using reverset_nat_equiv[OF List_list_wellbehaved[OF assms(1)], of "[] # ps" "[]"]
-    by (simp add: enc_List_list.simps)
-  done
-*)
-thm prefixes2_nat_equiv
 
 fun subtrees :: "'a tree \<Rightarrow> 'a tree list" where
   "subtrees \<langle>\<rangle> = []"
 | "subtrees \<langle>l, v, r\<rangle> = subtrees l @ subtrees r @ [l] @ [r]"
-
 
 function subtreest :: "'a tree \<Rightarrow> 'a tree list \<Rightarrow> 'a tree list \<Rightarrow> 'a tree list" where
   "subtreest \<langle>\<rangle> [] ts = ts"
@@ -483,7 +448,6 @@ lemma subtreest_correct: "mset (subtrees t) = mset (subtreest t [] [])"
   using subtrees_subtreest[of t "[]" "[]"] by simp
 
 function_nat_rewrite subtreest
-thm subtreest_nat.simps
 
 function_nat_rewrite_correctness subtreest
   by (natfn_correctness \<open>induct arg\<^sub>1 arg\<^sub>2 arg\<^sub>3 rule: subtreest.induct\<close>
@@ -493,14 +457,22 @@ function_nat_rewrite_correctness subtreest
       args_wellbehaved: encoding_tree_wellbehaved[OF assms(1), THEN pointfree_idE]
       encoding_list_wellbehaved[OF encoding_tree_wellbehaved, OF assms(1), THEN pointfree_idE])
 
-thm subtreest_nat_equiv
-
 
 
 
 
 
 (* TODOs/Things not wroking/Things to investigate *)
+
+
+fun fn_test1 :: "nat \<Rightarrow> nat" where
+  "fn_test1 x = (if x = 3 then 5 else 7)"
+
+fun fn_test2 :: "('a::order_bot) \<Rightarrow> nat" where
+  "fn_test2 a = 2"
+
+(* function_nat_rewrite fn_test1 *)
+(* function_nat_rewrite fn_test2 *)
 
 
 fun loop where
@@ -522,16 +494,16 @@ lemma loop_nat_equiv2:
   apply(all \<open>subst loop.simps\<close>)
   by(simp add: loop_nat.simps enc_list.simps)+
 
-fun rev where
-  "rev xs = loop [] xs"
+fun reverse where
+  "reverse xs = loop [] xs"
 
-function_nat_rewrite rev
-function_nat_rewrite_correctness rev
+function_nat_rewrite reverse
+function_nat_rewrite_correctness reverse
   using loop_nat_equiv[OF assms, of "[]"]
-  by (subst rev.simps, simp add: rev_nat.simps enc_list.simps)
+  by (subst reverse.simps, simp add: reverse_nat.simps enc_list.simps)
 
 fun append :: "'a list \<Rightarrow> 'a list \<Rightarrow> 'a list" where
-  "append xs ys = loop ys (rev xs)"
+  "append xs ys = loop ys (reverse xs)"
 
 
 lemma 2:"loop acc [x] = x # acc" by simp
@@ -560,28 +532,28 @@ lemma 7:"loop [] (loop [] xs) = xs"
   by (simp add: "4")
 
 lemma 8:"append xs ys = xs @ ys"
-  by (metis "3" "7" append.simps rev.simps)
+  by (metis "3" "7" append.simps reverse.simps)
 
 lemma 9:"rev (rev xs) = xs"
   by (simp add: "7")
 
-lemma 10:"rev (append xs ys) = append (rev ys) (rev xs)"
-  by (metis "4" "8" Encode_Nat.rev.simps append.elims)
+lemma 10:"reverse (append xs ys) = append (reverse ys) (reverse xs)"
+  by (metis "4" "8" Encode_Nat.reverse.simps append.elims)
 
-lemma rev_nat_equiv2:
+lemma reverse_nat_equiv2:
   assumes "dec_'a \<circ> enc_'a = id"
-  shows "rev_nat (enc_list enc_'a xs) = enc_list enc_'a (rev xs)"
-  apply(induction xs rule: rev.induct)
-  apply(subst rev.simps)
+  shows "reverse_nat (enc_list enc_'a xs) = enc_list enc_'a (reverse xs)"
+  apply(induction xs rule: reverse.induct)
+  apply(subst reverse.simps)
   using loop_nat_equiv2[OF assms]
-  by (metis "6" rev_nat.simps)
+  by (metis "6" reverse_nat.simps)
 
 function_nat_rewrite append
 function_nat_rewrite_correctness append
   apply(induction arg\<^sub>1 arg\<^sub>2 rule: append.induct)
   apply(all \<open>subst append.simps\<close>)
   apply(subst append_nat.simps)
-  using rev_nat_equiv2[OF assms] loop_nat_equiv[OF assms]
+  using reverse_nat_equiv2[OF assms(1)] loop_nat_equiv[OF assms]
   by(simp)
 
 lemma append_nat_equiv2:
@@ -589,7 +561,7 @@ lemma append_nat_equiv2:
   shows "append_nat (enc_list enc_'a xs) (enc_list enc_'a ys) = enc_list enc_'a (append xs ys)"
   apply(induction xs ys rule: append.induct)
   apply(subst append.simps)
-  using loop_nat_equiv2[OF assms] rev_nat_equiv2[OF assms]
+  using loop_nat_equiv2[OF assms] reverse_nat_equiv2[OF assms]
   using append_nat.simps by simp
 
 lemma append_nat_equiv3:
@@ -599,7 +571,7 @@ lemma append_nat_equiv3:
           = enc_list enc_'a (append xs (f ys))"
   apply(induction xs "f ys" rule: append.induct)
   apply(subst append.simps)
-  using loop_nat_equiv2[OF assms(1)] rev_nat_equiv2[OF assms(1)] assms(2)
+  using loop_nat_equiv2[OF assms(1)] reverse_nat_equiv2[OF assms(1)] assms(2)
   by (simp add: append_nat.simps)
 
 lemma append_nat_equiv4:
@@ -609,7 +581,7 @@ lemma append_nat_equiv4:
           = enc_list enc_'a (append (f xs) ys)"
   apply(induction "f xs" ys rule: append.induct)
   apply(subst append.simps)
-  using loop_nat_equiv2[OF assms(1)] rev_nat_equiv2[OF assms(1)] assms(2)
+  using loop_nat_equiv2[OF assms(1)] reverse_nat_equiv2[OF assms(1)] assms(2)
   by (simp add: append_nat.simps)
 
 lemma append_nat_equiv5:
@@ -620,7 +592,7 @@ lemma append_nat_equiv5:
           = enc_list enc_'a (append (f xs) (g ys))"
   apply(induction "f xs" "g ys" rule: append.induct)
   apply(subst append.simps)
-  using loop_nat_equiv2[OF assms(1)] rev_nat_equiv2[OF assms(1)] assms
+  using loop_nat_equiv2[OF assms(1)] reverse_nat_equiv2[OF assms(1)] assms
   by (simp add: append_nat.simps)
 
 
@@ -643,7 +615,7 @@ lemma 11:"prod_encode (0, 0) = enc_list enc_'a []"
 lemma "baz acc xs = baz2 acc xs"
   apply(induction xs arbitrary: acc)
   apply(simp)
-  by (metis (no_types, lifting) "7" append.elims atail.elims baz.simps(1) baz.simps(3) baz.simps(4) baz2.simps(1) baz2.simps(2) rev.elims)
+  by (metis (no_types, lifting) "7" append.elims atail.elims baz.simps(1) baz.simps(3) baz.simps(4) baz2.simps(1) baz2.simps(2) reverse.elims)
 
 
 
@@ -666,7 +638,7 @@ function_nat_rewrite_correctness baz2
   using encoding_list_wellbehaved[OF assms(1), THEN pointfree_idE]
   apply(simp add: baz2_nat.simps enc_list.simps)
   using encoding_list_wellbehaved[OF assms(1), THEN pointfree_idE]
-    baz2_nat_equiv2[OF assms]
+    baz2_nat_equiv2[OF assms(1)]
   by force
 
 lemma a: "(fstP (sndP (enc_list (enc_list enc_'a) [[]]))) = 0"
@@ -675,8 +647,8 @@ lemma a: "(fstP (sndP (enc_list (enc_list enc_'a) [[]]))) = 0"
 lemma b: "loop_nat 0 0 = 0"
   by(simp add: loop_nat.simps prod_decode_def prod_decode_aux.simps)
 
-lemma c: "rev_nat 0 = 0"
-  by(simp add: b rev_nat.simps prod_encode_def)
+lemma c: "reverse_nat 0 = 0"
+  by(simp add: b reverse_nat.simps prod_encode_def)
 
 lemma d: "append_nat 0 0 = 0"
   by(simp add: c b append_nat.simps)
@@ -715,20 +687,21 @@ lemma baz_nat_equiv2:
 
 
 lemma baz_nat_equiv2:
-  assumes "dec_'a \<circ> enc_'a = id"
+  assumes "(dec_'a :: pair_repr \<Rightarrow> ('a:: order_bot)) \<circ> enc_'a = id"
+    and "dec_'a bot = bot"
   shows "baz_nat (enc_list enc_'a acc) (enc_list (enc_list enc_'a) xss) = enc_list enc_'a (baz acc xss)"
   apply(induction acc xss rule: baz.induct)
   apply(all \<open>subst baz.simps\<close>)
   subgoal for acc
-    using append_nat_equiv2[OF assms] append_nat_equiv[OF assms]
-      append_nat_equiv3[OF assms] append_nat_equiv4[OF assms]
+    using append_nat_equiv2[OF assms(1)] append_nat_equiv[OF assms]
+      append_nat_equiv3[OF assms(1)] append_nat_equiv4[OF assms(1)]
     apply(simp add: Let_def)
     sorry
   subgoal by (metis "11" atomic.simps baz_nat.simps fstP.simps fst_conv prod_encode_inverse)
   subgoal sorry
   subgoal
     apply(subst baz_nat.simps)
-    using append_nat_equiv2[OF assms]
+    using append_nat_equiv2[OF assms(1)]
     sorry
   oops
 
@@ -741,7 +714,7 @@ function_nat_rewrite_correctness baz
 
     using encoding_list_wellbehaved[OF assms(1), THEN pointfree_idE]
       append_nat_equiv[OF assms]
-      append_nat_equiv2[OF assms]
+      append_nat_equiv2[OF assms(1)]
     sorry
   subgoal for acc
     using encoding_list_wellbehaved[OF assms(1), THEN pointfree_idE]
@@ -749,11 +722,11 @@ function_nat_rewrite_correctness baz
   subgoal premises IH for acc v va xss
 
     apply(subst IH[symmetric])
-    apply(subst append_nat_equiv2[OF assms, of acc "(v # va)", symmetric])
+    apply(subst append_nat_equiv2[OF assms(1), of acc "(v # va)", symmetric])
 
     using encoding_list_wellbehaved[OF assms(1), THEN pointfree_idE]
       append_nat_equiv[OF assms]
-      append_nat_equiv2[OF assms, of acc "(v # va)", symmetric]
+      append_nat_equiv2[OF assms(1), of acc "(v # va)", symmetric]
     sorry
   subgoal premises IH for acc xs v va
     apply(simp add: baz_nat.simps)
@@ -766,7 +739,7 @@ function_nat_rewrite_correctness baz
     apply(simp add: Let_def)
     using encoding_list_wellbehaved[OF assms(1), THEN pointfree_idE]
       append_nat_equiv[OF assms]
-      append_nat_equiv2[OF assms]
+      append_nat_equiv2[OF assms(1)]
       IH
     sorry
   done
